---
tags: 
Note Author:
  - Trym A. Gabrielsen
Theory Author: 
Reviewed By:
---
$$x^{ref}(t),~~ u^{ref}(t)\quad \forall t\in[0,T]$$$$\begin{align*}
x^{ref} = \{x^{ref}_{0},x^{ref}_{1},x^{ref}_{2},~\dots~,x^{ref}_{N-1},x^{ref}_{N}\}\\
u^{ref} = \{u^{ref}_{0},u^{ref}_{1},u^{ref}_{2},~\dots~,u^{ref}_{N-1},u^{ref}_{N}\}
\end{align*}$$where $$x_{i}^{ref} = x^{ref}(t_{i}), \quad u_{i}^{ref} = u^{ref}(t_{i})$$$$\begin{align*}
x^{ref,i} = \{x^{ref}_{i},x^{ref}_{i+1},~\dots~,x^{ref}_{i+H-1},x^{ref}_{i+H}\}\\
u^{ref,i} = \{u^{ref}_{i},u^{ref}_{i+1},~\dots~,u^{ref}_{i+H-1},u^{ref}_{i+H}\}
\end{align*}$$such that $$x^{ref,i}_{j} = x^{ref}_{i+j}, \quad u^{ref,i}_{j} = u^{ref}_{i+j}$$
